cfi/preservation.v
@@ -1,5 +1,5 @@
 Require Import Coq.Lists.List Coq.Bool.Bool.
-Require Import common.common. 
+Require Import common.common.
 Require Import lib.utils lib.Coqlib.
 Require Import cfi.property.
 
@@ -7,9 +7,9 @@ Set Implicit Arguments.
 
 Import ListNotations.
 
-(* Refinement for two generic (cfi) machines *)
+(* CFI preserved by refinement for two generic (cfi) machines *)
 
-Section Refinement.
+Section Preservation.
 
 Context {t : machine_types}
         {ops : machine_ops t}
@@ -25,18 +25,20 @@ Variable CS : (list (@state cmachine)) -> Prop.
 (* General notion of refinement between two machines*)
 Class machine_refinement (amachine : cfi_machine) (cmachine : cfi_machine) := {
   refine_state : (@state amachine) -> (@state cmachine) -> Prop;
- 
-  visible : (@state cmachine) -> (@state cmachine) -> bool;
 
-  backwards_refinement_normal :  
+  check : (@state cmachine) -> (@state cmachine) -> bool;
+
+  backwards_refinement_normal :
     forall ast cst cst'
       (REF: refine_state ast cst)
       (STEP: step cst cst'),
-      (visible cst cst' = true ->
+      (check cst cst' = true ->
        exists ast', step ast ast' /\ refine_state ast' cst')
-      /\ (visible cst cst' = false -> refine_state ast cst');
+      /\ (check cst cst' = false ->
+          refine_state ast cst' \/
+          exists ast', step ast ast' /\ refine_state ast' cst');
 
-  backwards_refinement_attacker :  
+  backwards_refinement_attacker :
     forall ast cst cst'
       (REF: refine_state ast cst)
       (STEPA: step_a cst cst'),
@@ -48,19 +50,18 @@ Context (rf : machine_refinement amachine cmachine).
 
 Inductive refine_traces :
   list (@state amachine) -> list (@state cmachine) -> Prop :=
-| TRNil : forall ast cst, 
-            refine_state ast cst -> 
+| TRNil : forall ast cst,
+            refine_state ast cst ->
             refine_traces [ast] [cst]
 | TRNormal0 : forall ast cst cst' axs cxs,
     step cst cst' ->
-    visible cst cst' = false ->
+    check cst cst' = false ->
     refine_state ast cst ->
     refine_state ast cst' ->
     refine_traces (ast :: axs) (cst' :: cxs) ->
     refine_traces (ast :: axs) (cst :: cst' :: cxs)
 | TRNormal1 : forall ast ast' cst cst' axs cxs,
     step cst cst' ->
-    visible cst cst' = true ->
     step ast ast' ->
     refine_state ast cst ->
     refine_state ast' cst' ->
@@ -85,9 +86,9 @@ Class machine_refinement_specs := {
     initial cst ->
     exists (ast : @state amachine), initial ast /\ refine_state ast cst;
 
-  cfg_invisible : forall csi csj, 
+  cfg_nocheck : forall csi csj,
     step csi csj ->
-    visible csi csj = false ->
+    check csi csj = false ->
     succ csi csj = true;
 
   cfg_equiv : forall (asi asj : @state amachine) csi csj,
@@ -107,12 +108,14 @@ Class machine_refinement_specs := {
     refine_state ast cst ->
     refine_state ast' cst' ->
     succ ast ast' = false ->
-    visible cst cst' = true ->
+    check cst cst' = true ->
     succ cst cst' = false;
 
   (* Q: Can this be simplified to if we were to show that
      backwards_refinement_traces_stronger produces _unique_ axs?
      Doesn't seem easy to state! *)
+  (* CH: not clear how possible it was before, but this is clearly not
+     possible with the new way to define backwards_refinement_normal *)
   as_implies_cs : forall axs cxs,
     refine_traces axs cxs ->
     AS axs ->
@@ -138,15 +141,23 @@ Proof.
   {
     destruct (step_classic cst cst') as [STEPN | NST].
   - destruct (backwards_refinement_normal _ _ _ INITREF STEPN) as [VIS INVIS].
-    destruct (visible cst cst') eqn:VISIBLE.
+    destruct (check cst cst') eqn:CHECK.
     + destruct (VIS eq_refl) as [ast' [ASTEP AREF]]. clear INVIS VIS.
       exists [ast;ast']. split.
       * exists ast'. eapply intermr_multi. right. eassumption. now constructor.
       * apply TRNormal1; auto.
         constructor(assumption).
     + specialize (INVIS eq_refl); clear VIS.
-      exists [ast]; split; [exists ast; constructor | apply TRNormal0; auto].
-      now constructor(assumption).
+      destruct INVIS as [ZERO | [ast' [STEP REF]]].
+      * exists [ast]; split; [exists ast; constructor | apply TRNormal0; auto].
+        now constructor(assumption).
+      * exists [ast; ast'].
+        { split.
+          - exists ast'.
+            econstructor; first by (right; eauto).
+            constructor.
+          - apply TRNormal1; eauto.
+            by constructor. }
   - destruct STEP2 as [STEP2A | STEP2N]; [idtac | tauto].
     destruct (backwards_refinement_attacker _ _ _ INITREF STEP2A) as [ast' [STEPA REF]].
     exists [ast;ast']; split;
@@ -155,7 +166,7 @@ Proof.
   }
   { destruct (step_classic cst cst'') as [STEPN | NST].
     - destruct (backwards_refinement_normal _ _ _ INITREF STEPN) as [VIS INVIS].
-      destruct (visible cst cst'') eqn:VISIBLE.
+      destruct (check cst cst'') eqn:CHECK.
       + destruct (VIS eq_refl) as [ast'' [ASTEP AREF]]. clear INVIS VIS.
         destruct (IHINTERM2' ast'' AREF) as [axs [[ast' INTERMR1] IH]].
         exists (ast :: axs); split.
@@ -167,49 +178,60 @@ Proof.
         * apply intermr_first_step in INTERMR1; apply interm_first_step in INTERM2';
           subst.
           apply TRNormal1; auto.
-      + (*invisible step case*)
+      + (*nocheck step case*)
         specialize (INVIS eq_refl); clear VIS.
-        destruct (IHINTERM2' ast INVIS) as [axs [[ast' INTERMR1] IH]].
-        exists axs. split.
-        exists ast'; now assumption.
-        destruct axs; 
-          [inversion INTERMR1 | apply intermr_first_step in INTERMR1; subst].
-        destruct cxs'; 
-          [inversion INTERM2' | apply interm_first_step in INTERM2'; subst].
-        apply TRNormal0; auto.
+        destruct INVIS as [ZERO | [ast' [STEP REF]]].
+        * destruct (IHINTERM2' ast ZERO) as [axs [[ast' INTERMR1] IH]].
+          exists axs. split.
+          exists ast'; now assumption.
+          destruct axs;
+            [inversion INTERMR1 | apply intermr_first_step in INTERMR1; subst].
+          destruct cxs';
+            [inversion INTERM2' | apply interm_first_step in INTERM2'; subst].
+          apply TRNormal0; auto.
+        * destruct (IHINTERM2' _ REF) as [axs [[ast'' INTERMR1] IH]].
+          exists (ast :: axs).
+          { split.
+            - exists ast''. econstructor; eauto. by right.
+            - destruct axs; first by inversion IH.
+              destruct cxs'; first by inversion IH.
+              apply interm_first_step in INTERM2'. subst.
+              apply intermr_first_step in INTERMR1. subst.
+              by eapply TRNormal1; eauto. }
       + destruct STEP2 as [STEP2A | STEP2N]; subst.
         { (*case it's an attacker step*)
-          destruct (backwards_refinement_attacker _ _ _ INITREF STEP2A) 
+          destruct (backwards_refinement_attacker _ _ _ INITREF STEP2A)
           as [ast'' [ASTEP REF]].
         destruct (IHINTERM2' _ REF) as [axs [[ast' INTERMR1] IH]].
         exists (ast::axs).
-        split. exists ast'. eapply intermr_multi; eauto. 
+        split. exists ast'. eapply intermr_multi; eauto.
         left; now assumption.
-        destruct axs; 
+        destruct axs;
           [inversion INTERMR1 | apply intermr_first_step in INTERMR1; subst].
-        destruct cxs'; 
+        destruct cxs';
           [inversion INTERM2' | apply interm_first_step in INTERM2'; subst].
         apply TRAttacker; auto.
         }
         { (*case it's a normal step*)
-          tauto. 
+          tauto.
         }
   }
 Qed.
-  
+
+(*
 Lemma refine_traces_weaken_backward : forall axs cxs,
   refine_traces axs cxs ->
     (forall csi csj,
        In2 csi csj cxs ->
        step csi csj ->
-       visible csi csj = true ->
+       check csi csj = true ->
          exists asi asj,
            In2 asi asj axs /\ step asi asj
            /\ refine_state asi csi /\ refine_state asj csj).
 Proof.
-  intros axs cxs RTRACE csi csj IN2 CSTEP VISIBLE.
-  induction RTRACE 
-    as [ast cst REF | ast cst cst' axs' cxs' STEP VIS ASTEP' REF REF' RTRACE' | 
+  intros axs cxs RTRACE csi csj IN2 CSTEP CHECK.
+  induction RTRACE
+    as [ast cst REF | ast cst cst' axs' cxs' STEP VIS ASTEP' REF REF' RTRACE' |
         ast ast' cst cst' axs cxs STEP VIS ASTEP' REF REF' RTRACE'|
         ast ast' cst cst' axs cxs NSTEP STEP ASTEP' REF REF' RTRACE']; subst.
   - destruct IN2.
@@ -239,12 +261,12 @@ Lemma refine_traces_weaken_forward : forall axs cxs,
     step asi asj ->
     succ asi asj = false ->
     exists csi csj,
-      In2 csi csj cxs /\ step csi csj /\ visible csi csj = true
+      In2 csi csj cxs /\ step csi csj /\ check csi csj = true
       /\ refine_state asi csi /\ refine_state asj csj.
 Proof.
   intros axs cxs RTRACE asi asj IN2 ASTEP SUCC.
-  induction RTRACE 
-    as [ast cst REF | ast cst cst' axs' cxs' STEP VIS ASTEP' REF REF' RTRACE' | 
+  induction RTRACE
+    as [ast cst REF | ast cst cst' axs' cxs' STEP VIS ASTEP' REF REF' RTRACE' |
         ast ast' cst cst' axs cxs STEP VIS ASTEP' REF REF' RTRACE'|
         ast ast' cst cst' axs cxs NSTEP STEP ASTEP' REF REF' RTRACE']; subst.
   - destruct IN2.
@@ -264,13 +286,14 @@ Proof.
       repeat (split; auto).
   - destruct IN2 as [[? ?] | IN2]; subst.
     * destruct (av_no_attacker _ _ SUCC ASTEP). now assumption.
-    * apply IHRTRACE' in IN2. 
+    * apply IHRTRACE' in IN2.
       destruct IN2 as [csi [csj [IN2' [STEPN [REFI REFJ]]]]].
       exists csi; exists csj.
       split. change (cst :: cst' :: cxs) with ([cst] ++ (cst' :: cxs)).
       apply in2_strengthen. now assumption.
       repeat (split; auto).
 Qed.
+*)
 
 Lemma refine_traces_preserves_cfi_trace : forall axs cxs,
   refine_traces axs cxs ->
@@ -278,35 +301,35 @@ Lemma refine_traces_preserves_cfi_trace : forall axs cxs,
   trace_has_cfi cmachine cxs.
 Proof.
   intros axs cxs RTRACE TSAFE csi csj IN2 CSTEP.
-  induction RTRACE 
-    as [ast cst REF | ast cst cst' axs' cxs' STEP VIS ASTEP' REF RTRACE' | 
-        ast ast' cst cst' axs cxs STEP VIS ASTEP' REF REF' RTRACE'|
+  induction RTRACE
+    as [ast cst REF | ast cst cst' axs' cxs' STEP VIS ASTEP' REF RTRACE' |
+        ast ast' cst cst' axs cxs STEP ASTEP' REF REF' RTRACE'|
         ast ast' cst cst' axs cxs NSTEP STEP ASTEP' REF REF' RTRACE']; subst.
   - destruct IN2.
   - destruct IN2 as [[? ?] | IN2]; subst.
-    * apply (cfg_invisible _ _ CSTEP VIS).
+    * apply (cfg_nocheck _ _ CSTEP VIS).
     * apply IHRTRACE'; assumption.
   - destruct IN2 as [[? ?] | IN2]; subst.
     * assert (SUCC: succ ast ast' = true).
       { apply TSAFE; simpl; auto. }
       apply (cfg_equiv _ _ _ _ REF REF' SUCC).
-    * apply IHRTRACE'. 
+    * apply IHRTRACE'.
       destruct axs.
       + intros ? ? CONTRA; destruct CONTRA.
       + intros asi asj IN2'. unfold trace_has_cfi in TSAFE.
-        apply in2_strengthen with (ys := [ast]) in IN2'. 
-        change ([ast] ++ ast' :: s :: axs ) 
+        apply in2_strengthen with (ys := [ast]) in IN2'.
+        change ([ast] ++ ast' :: s :: axs )
         with (ast :: ast' :: s :: axs) in IN2'.
         apply TSAFE. now assumption.
         now assumption.
   - destruct IN2 as [[? ?] | IN2]; subst.
     * tauto.
-    * apply IHRTRACE'. 
+    * apply IHRTRACE'.
       destruct axs.
       + intros ? ? CONTRA; destruct CONTRA.
       + intros asi asj IN2'. unfold trace_has_cfi in TSAFE.
-        apply in2_strengthen with (ys := [ast]) in IN2'. 
-        change ([ast] ++ ast' :: s :: axs ) 
+        apply in2_strengthen with (ys := [ast]) in IN2'.
+        change ([ast] ++ ast' :: s :: axs )
         with (ast :: ast' :: s :: axs) in IN2'.
         apply TSAFE. now assumption.
         now assumption.
@@ -319,7 +342,7 @@ Lemma refine_traces_split axs ahd atl asi asj cxs :
   succ asi asj = false ->
   exists chd csi csj ctl,
     step csi csj /\
-    visible csi csj = true /\
+    (*check csi csj = true /\*)
     refine_state asi csi /\
     refine_state asj csj /\
     refine_traces (ahd ++ [asi]) (chd ++ [csi]) /\
@@ -330,7 +353,7 @@ Proof.
   gdep viol. gdep astep. gdep ahd. gdep asi. gdep asj. gdep atl.
   induction ref; intros.
   - by repeat (destruct ahd; inversion eqaxs).
-  - edestruct IHref as [chd [csi [csj [ctl [CSTEP [VIS [REFI [REFJ [RTHD [RTT CLST]]]]]]]]]]; eauto.
+  - edestruct IHref as [chd [csi [csj [ctl [CSTEP [REFI [REFJ [RTHD [RTT CLST]]]]]]]]]; eauto.
     exists (cst :: chd); repeat eexists; eauto. simpl.
     destruct chd; destruct ahd; simpl in *; inv CLST; inv eqaxs; apply TRNormal0; eauto.
     rewrite CLST. reflexivity.
@@ -339,28 +362,34 @@ Proof.
       exists []. exists cst. exists cst'. exists cxs.
       repeat split; eauto. by constructor(assumption).
     + inv eqaxs.
-      edestruct IHref as [chd [csi [csj [ctl [CSTEP [VIS [REFI [REFJ [RTHD [RTT CLST]]]]]]]]]]; eauto.
+      edestruct IHref as [chd [csi [csj [ctl [CSTEP [REFI [REFJ [RTHD [RTT CLST]]]]]]]]]; eauto.
       clear IHref.
       exists (cst :: chd). exists csi. exists csj. exists ctl.
-      repeat split; eauto. 
-      * destruct chd; destruct ahd; simpl in *; inv CLST; inv H6;
+      repeat split; eauto.
+      * destruct chd; destruct ahd; simpl in *; inv CLST; inv H5;
          apply TRNormal1; eauto.
         rewrite CLST. reflexivity.
   - destruct ahd; simpl in *; inv eqaxs.
     apply False_ind. by eapply av_no_attacker; eauto.
-    edestruct IHref as [chd [csi [csj [ctl [CSTEP [VIS [REFI [REFJ [RTHD [RTT CLST]]]]]]]]]]; eauto.
+    edestruct IHref as [chd [csi [csj [ctl [CSTEP [REFI [REFJ [RTHD [RTT CLST]]]]]]]]]; eauto.
     exists (cst :: chd); repeat eexists; eauto. simpl.
     destruct chd; destruct ahd; simpl in *; inv CLST; inv H6;
     apply TRAttacker; eauto.
     rewrite CLST. reflexivity.
-Qed.   
+Qed.
 
 (*Preservation Theorem*)
 
+Lemma In2_inv {X} xs xmid xs' (x1 x2 : X) :
+  In2 x1 x2 (xs ++ xmid :: xs') ->
+  In2 x1 x2 (xs ++ [xmid]) \/
+  In2 x1 x2 (xmid :: xs').
+Admitted.
+
 Theorem backwards_refinement_preserves_cfi :
   cfi amachine AS ->
-  cfi cmachine CS. 
-Proof. 
+  cfi cmachine CS.
+Proof.
   intros CFI1 cst cst' cxs INIT2 INTERM2.
   destruct (initial_refine cst INIT2) as [ast [INIT1 INITREF]].
   destruct (backwards_refinement_traces_stronger ast INITREF INTERM2)
@@ -372,18 +401,27 @@ Proof.
     - (*machine1 has CFI at all steps*)
       left. apply (refine_traces_preserves_cfi_trace RTRACE TSAFE1).
     - (*machine1 has a violation*)
-      destruct VIOLATED 
+      destruct VIOLATED
          as [asi [asj [ahs [atl [ALST [[ASTEP AV] [TSAFE1 [TSAFE2 STOP1]]]]]]]].
-      right.
       assert (IN2: In2 asi asj axs) by (rewrite ALST; apply in2_trivial).
-      destruct (refine_traces_split ahs atl asi asj ALST RTRACE ASTEP AV) 
-        as [chs [csi [csj [ctl [CSTEP [VIS [REFI [REFJ [RHT [RTT CLST]]]]]]]]]].
-      exists csi; exists csj; exists chs; exists ctl.
-      split. now assumption.
-      split. split; [assumption | apply (av_implies_cv asi asj csi csj REFI REFJ AV VIS)].
-      split. now apply (refine_traces_preserves_cfi_trace RHT TSAFE1).
-      split. now apply (refine_traces_preserves_cfi_trace  RTT TSAFE2).
-      apply (as_implies_cs RTT STOP1).
+      destruct (refine_traces_split ahs atl asi asj ALST RTRACE ASTEP AV)
+        as [chs [csi [csj [ctl [CSTEP [REFI [REFJ [RHT [RTT CLST]]]]]]]]].
+      destruct (check csi csj) eqn:VIS.
+      + right.
+        exists csi; exists csj; exists chs; exists ctl.
+        split. now assumption.
+        split. split; [assumption | apply (av_implies_cv asi asj csi csj REFI REFJ AV VIS)].
+        split. now apply (refine_traces_preserves_cfi_trace RHT TSAFE1).
+        split. now apply (refine_traces_preserves_cfi_trace  RTT TSAFE2).
+        apply (as_implies_cs RTT STOP1).
+      + left.
+        intros csi' csj' IN2' STEP'.
+        subst cxs.
+        apply In2_inv in IN2'.
+        destruct IN2' as [IN2' | [[E1 E2] | IN2']].
+        * by apply (refine_traces_preserves_cfi_trace RHT TSAFE1).
+        * subst. by eauto using cfg_nocheck.
+        * by apply (refine_traces_preserves_cfi_trace  RTT TSAFE2).
   }
   { (*machine1 no step*)
     subst. left.
@@ -397,10 +435,10 @@ Proof.
     - destruct IN2.
     - destruct IN2 as [[? ?] | IN2]; subst.
       * inversion RTRACE; subst.
-        apply (cfg_invisible _ _ H4 H5).
+        apply (cfg_nocheck _ _ H4 H5).
       * inversion RTRACE; subst.
-        now apply (IHcxs _ H8 IN2). 
+        now apply (IHcxs _ H8 IN2).
   }
 Qed.
 
-End Refinement.
+End Preservation.
